Coq/Coq23.v
@@ -1,0 +1,26 @@
+Module Coq23.
+
+  Inductive strange : Set :=
+    cs : strange -> strange.
+
+  Lemma silly : forall x : strange, cs x = x.
+Proof.
+  intros.
+  induction x. rewrite IHx. auto.
+Qed.
+  Lemma strange_equ : forall x y : strange, x = y.
+ Proof.
+    intros. induction x.
+    destruct y.
+    rewrite <- IHx. apply silly.
+Qed.
+
+ Inductive A : Prop :=
+   base : Set -> A
+ | succ' : A -> A.
+
+ Require Import Nat.
+ Require Import Arith.
+
+ Check (succ' (base nat)).
+ 
