Coq/Coq24.v
@@ -1,0 +1,5 @@
+(*
+  Exercises for <Software Foundations> V2 CH2.
+  Arthur : Brethland, Late 2019.
+ *)
+
