Agda/Ag01.agda
@@ -1,0 +1,11 @@
+module Ag01 where
+
+-- open import Agda.Builtin.Nat
+
+
+data ℕ : Set where
+  zero : ℕ
+  succ : ℕ → ℕ
+
+{-# BUILTIN NATURAL ℕ #-}
+
